Db/Model/Meta/Attribute.lean
@@ -1,0 +1,33 @@
+/-
+Copyright (c) 2025 Christian Merten. All rights reserved.
+Released under Apache 2.0 license as described in the file LICENSE.
+Authors: Christian Merten
+-/
+import Lean.Elab.Command
+
+open Lean Elab
+
+structure ModelTag where
+  declName : Name
+  -- TODO: add meta information
+  deriving DecidableEq, Hashable
+
+initialize tagExt : SimplePersistentEnvExtension ModelTag (Std.HashSet ModelTag) ←
+  registerSimplePersistentEnvExtension {
+    addImportedFn := fun as => as.foldl Std.HashSet.insertMany {}
+    addEntryFn := .insert
+  }
+
+def addModelTag {m : Type → Type} [MonadEnv m] (tag : ModelTag) : m Unit :=
+  modifyEnv (tagExt.addEntry · tag)
+
+syntax (name := modelTag) "model" : attr
+
+initialize Lean.registerBuiltinAttribute {
+  name := `modelTag
+  descr := "Tag a structure with a model tag"
+  add decl stx _ := do
+    match stx with
+    | `(attr| model) => addModelTag { declName := decl }
+    | _ => throwUnsupportedSyntax
+}
