Db/Model/Meta/GenerateTable.lean
@@ -1,0 +1,183 @@
+/-
+Copyright (c) 2025 Christian Merten. All rights reserved.
+Released under Apache 2.0 license as described in the file LICENSE.
+Authors: Christian Merten
+-/
+import Lean.Elab.Tactic.Meta
+import Lean.Elab.Command
+import Lean.Elab.Deriving.Basic
+import Lean.Meta.Constructions.CtorIdx
+import Lean.Meta.Constructions.CasesOn
+import Db.Query.Basic
+import Db.Utils.Equiv
+
+open Lean Elab Command
+
+def Lean.Expr.getForallArgs : Expr → List (Name × Expr)
+  | .forallE n t b _ => (n, t) :: getForallArgs b
+  | _ => []
+
+syntax (name := generateTableStx) "generate_table " ident : command
+
+def getStructureArgs {m : Type → Type} [Monad m] [MonadEnv m] [MonadError m] (decl : Name) :
+    m (List (Name × Expr)) := do
+  let .inductInfo info := ← getConstInfo decl | throwError "Not a structure."
+  unless info.ctors.length == 1 do throwError "Not a structure."
+  let ctor := info.ctors[0]!
+  let ctorInfo ← getConstInfo ctor
+  return ctorInfo.type.getForallArgs
+
+def mkEnumDeclaration (name : Name) (names : List Name) : Declaration :=
+  Lean.mkInductiveDeclEs [] 0 [
+    { name := name
+      type := .sort 1
+      ctors := names.map fun arg ↦ { name := name ++ arg, type := .const name [] } }
+  ] false
+
+def fromEnum (name : Name) (expr : Array Expr) (type : Expr) : MetaM Expr := do
+  let motive : Expr ← Meta.withLocalDecl `x BinderInfo.default (.const name []) fun x => do
+    Meta.mkLambdaFVars #[x] type
+  Meta.withLocalDecl `x BinderInfo.default (.const name []) fun x => do
+    let body ← Meta.mkAppOptM (name ++ `casesOn) (#[some motive, some x] ++ (expr.map Option.some))
+    Meta.mkLambdaFVars #[x] body
+
+def FromString.ofToString (α : Type) [ToString α] [Enum α] : FromString α where
+  fromString s := Id.run do
+    let mut res : Option α := none
+    for x in Enum.all α do
+      if s == toString x then
+        res := some x
+    return res
+
+def List.toExpr (type : Expr) : List Expr → MetaM Expr
+  | [] => Meta.mkAppOptM ``List.nil #[some type]
+  | e :: es => do Meta.mkAppM ``List.cons #[e, ← es.toExpr type]
+
+def elabInstance (expr : Expr) : CommandElabM Unit := do
+  let instName : Name ← Lean.mkAuxDeclName
+  let instDecl : Declaration := .defnDecl
+    { name := instName
+      levelParams := []
+      type := ← liftTermElabM <| Meta.inferType expr
+      value := expr
+      hints := default
+      safety := .safe }
+  liftCoreM <| addAndCompile instDecl
+  liftTermElabM <| Meta.addInstance instName default 1000
+
+def mkMatch (var : Expr) (default : Expr) : List (Expr × Expr) → MetaM Expr
+  | [] => pure default
+  | (comp, val) :: xs => do
+    Meta.mkAppM
+      ``cond #[← Meta.mkAppM ``BEq.beq #[var, comp], val, ← mkMatch var default xs]
+
+def elabEnum (name : Name) (names : List (Name × String)) : CommandElabM Unit := do
+  let decl : Declaration :=
+    mkEnumDeclaration name (names.map Prod.fst)
+  liftCoreM <| addAndCompile decl
+  liftTermElabM <| do
+    mkCasesOn name
+    mkCtorIdx name
+  applyDerivingHandlers ``DecidableEq #[name]
+  applyDerivingHandlers ``Hashable #[name]
+  let toString : Expr ← liftTermElabM <| do
+    let val : Expr ←
+      fromEnum name (names.toArray.map fun x ↦ .lit <| .strVal x.2) (.const ``String [])
+    Meta.mkAppM ``ToString.mk #[val]
+  elabInstance toString
+  let enum : Expr ← liftTermElabM <| do
+    let arr : Expr ← Meta.mkAppM ``Array.mk
+      #[← (names.map fun x ↦ .const (name ++ x.1) []).toExpr (.const name [])]
+    let val : Expr ←
+      Meta.mkAppOptM ``Std.HashSet.ofArray
+        #[Expr.const name [], none, none, arr]
+    Meta.mkAppM ``Enum.mk #[val]
+  elabInstance enum
+  let fromString : Expr ← liftTermElabM <| do
+    -- Meta.mkAppM ``FromString.ofToString #[.const name []]
+    let val : Expr ←
+      Meta.withLocalDecl `x BinderInfo.default (.const ``String []) fun x => do
+        let body : Expr ← do
+          mkMatch
+            x
+            (← Meta.mkAppOptM ``Option.none #[Expr.const name []])
+            (← names.mapM fun y => do pure (.lit <| .strVal y.2,
+              ← Meta.mkAppM ``Option.some #[.const (name ++ y.1) []]))
+        Meta.mkLambdaFVars #[x] body
+    Meta.mkAppM ``FromString.mk #[val]
+  elabInstance fromString
+  let indexing : Expr ← liftTermElabM <| do
+    let app ← Meta.mkAppOptM ``Indexing.mk #[Expr.const name [],
+      none, none, none]
+    match (← Meta.inferType app).getForallArgs with
+    | [(_name, type)] =>
+      let e ← Meta.mkFreshExprMVar type
+      _ ← Elab.runTactic e.mvarId! (← `(tactic| intro x; induction x <;> rfl))
+      Meta.mkAppM' app #[e]
+    | vars =>
+      logInfo s!"{vars}"
+      return app
+  elabInstance indexing
+
+class HasDBType (α : Type) where
+  dbType : DBType
+  encoding : α ≃ dbType.Value
+
+instance : HasDBType Bool where
+  dbType := .bool
+  encoding := Equiv.refl _
+
+instance (n : Nat) : HasDBType (VarChar n) where
+  dbType := .varchar n
+  encoding := Equiv.refl _
+
+instance : HasDBType Int where
+  dbType := .int
+  encoding := Equiv.refl _
+
+/-- Generate a `Table` for structure named `decl`. -/
+def generateTable (decl : Name) : CommandElabM Unit := do
+  let names ← getStructureArgs decl
+  let indexName : Name := (s!"{decl}Index").toName
+  let tableName : Name := (s!"{decl}Table").toName
+  -- Add indexing type
+  elabEnum indexName (names.map fun x ↦ (x.1, x.1.toString))
+  -- Construct `Index → Column`
+  let cols : Array Expr ← liftTermElabM <|
+    names.toArray.mapM fun (_, type) ↦ do
+      let dbtype : Expr ← Meta.mkAppOptM ``HasDBType.dbType #[some type, none]
+      Meta.mkAppM ``Column.mk
+        #[dbtype, .const ``Bool.false []]
+  let colMap : Expr ←
+    liftTermElabM <| fromEnum indexName cols (.const ``Column [])
+  -- Construct `Table` and add to environment
+  let table : Expr ← liftTermElabM <|
+    Meta.mkAppM ``Table.mk #[.const indexName [], colMap]
+  let tableDecl : Declaration :=
+    .defnDecl
+      { name := tableName
+        levelParams := []
+        type := .const ``Table []
+        value := table
+        hints := default
+        safety := .safe }
+  liftCoreM <| addAndCompile tableDecl
+
+@[command_elab generateTableStx]
+def generateTableElab : CommandElab
+  | `(command| generate_table $decl) => generateTable decl.getId
+  | _ => throwUnsupportedSyntax
+
+section Example
+
+structure Baz where
+  val : Bool
+  name : VarChar 10
+  val2 : Int
+
+generate_table Baz
+
+example : (BazTable.columns .val).type = .bool := rfl
+example : (BazTable.columns .val2).type = .int := rfl
+
+end Example
