Db/Utils/Enum.lean
@@ -1,0 +1,9 @@
+import Std
+
+universe u
+
+class Enum (α : Type u) : Type u extends Hashable α where
+  [decidableEq : DecidableEq α]
+  all (α) : Std.HashSet α
+
+attribute [instance] Enum.decidableEq
