Db/Utils/Equiv.lean
@@ -7,3 +7,9 @@ structure Equiv (α : Type u) (β : Type v) where
   toFun_invFun (b : β) : toFun (invFun b) = b
 
 notation α:max " ≃ " β:max => Equiv α β
+
+def Equiv.refl (α : Type u) : α ≃ α where
+  toFun := id
+  invFun := id
+  invFun_toFun := by grind
+  toFun_invFun := by grind
